theories/Terms.v
@@ -23,6 +23,9 @@ Inductive term : Set :=
   | TmInl (e : term)
   | TmInr (e : term)
   | TmPlusCase (eta : env) (r : type) (z : string) (x : string) (e1 : term) (y : string) (e2 : term)
+  | TmNil
+  | TmCons (e : term) (e' : term)
+  | TmStarCase (eta : env) (r : type) (z : string) (e1 : term) (x : string) (xs : string) (e2 : term)
   | TmFix (args : argsterm) (hpargs : histargs) (g : context) (r : type) (e : term)
   | TmRec (args : argsterm) (hpargs : histargs)
   | TmArgsLet (args : argsterm) (g : context) (e : term)
@@ -50,6 +53,9 @@ Fixpoint fix_subst (g : context) (r : type) (e : term) (e' : term) :=
   | TmInl e' => TmInl (fix_subst g r e e')
   | TmInr e' => TmInr (fix_subst g r e e')
   | TmPlusCase eta r' z x e1 y e2 => TmPlusCase eta r' z x (fix_subst g r e e1) y (fix_subst g r e e2)
+  | TmNil => TmNil
+  | TmCons e1 e2 => TmCons (fix_subst g r e e1) (fix_subst g r e e2)
+  | TmStarCase eta r' z e1 x xs e2 => TmStarCase eta r' z (fix_subst g r e e1) x xs (fix_subst g r e e2)
   | TmFix args hpargs g' r' e' => TmFix (fix_subst_args g r e args) hpargs g' r' e'
   | TmRec args hpargs => TmFix (fix_subst_args g r e args) hpargs g r e
   | TmArgsLet args g' e' => TmArgsLet (fix_subst_args g r e args) g' (fix_subst g r e e')
@@ -84,6 +90,9 @@ Fixpoint histval_subst (v : histval) (n : nat) (e : term) :=
   | TmInl e' => TmInl (histval_subst v n e')
   | TmInr e' => TmInr (histval_subst v n e')
   | TmPlusCase eta r' z x e1 y e2 => TmPlusCase eta r' z x (histval_subst v n e1) y (histval_subst v n e2)
+  | TmNil => TmNil
+  | TmCons e1 e2 => TmCons (histval_subst v n e1) (histval_subst v n e2)
+  | TmStarCase eta r' z e1 x xs e2 => TmStarCase eta r' z (histval_subst v n e1) x xs (histval_subst v n e2)
   | TmFix args hpargs g' r' e' => TmFix (histval_subst_args v n args) (histval_subst_histargs v n hpargs) g' r' e'
   | TmRec args hpargs => TmRec (histval_subst_args v n args) (histval_subst_histargs v n hpargs)
   | TmArgsLet args g' e' => TmArgsLet (histval_subst_args v n args) g' (histval_subst v n e')
@@ -142,14 +151,15 @@ Hint Resolve eqb_spec_term : core.
  *)
 Fixpoint fv_term e : set string :=
   match e with
-  | TmSink | TmUnit => empty_set
+  | TmSink | TmUnit | TmNil => empty_set
   | TmVar x => singleton_set x
-  | TmComma e1 e2 | TmSemic e1 e2 => set_union (fv_term e1) (fv_term e2)
+  | TmComma e1 e2 | TmSemic e1 e2 | TmCons e1 e2 => set_union (fv_term e1) (fv_term e2)
   | TmLetPar x y z e | TmLetCat _ x y z e => set_union (singleton_set z) (
       set_minus (set_minus (fv_term e) (singleton_set x)) (singleton_set y))
   | TmLet x e e' => set_union (fv_term e) (set_minus (fv_term e') (singleton_set x))
   | TmInl e | TmInr e => fv_term e
   | TmPlusCase _ _ z x e1 y e2 => set_union (singleton_set z) (set_union (set_minus (fv_term e1) (singleton_set x)) (set_minus (fv_term e2) (singleton_set y)))
+  | TmStarCase _ _ z e1 x xs e2 => set_union (singleton_set z) (set_union (fv_term e1) (set_minus (fv_term e2) (set_union (singleton_set x) (singleton_set xs))))
   | TmFix args _ _ _ _ => fv_argsterm args
   | TmRec args _ => fv_argsterm args
   | TmArgsLet args _ _ => fv_argsterm args
